fairness/examples/spinlock/spinlock_sc_adequacy.v
@@ -352,11 +352,12 @@ Theorem spinlock_terminates
         (Hexfirst : (trfirst extr).1 = [program #()]):
   (∀ tid, fair_ex tid extr) -> terminating_trace extr.
 Proof.
-  set (Σ := gFunctors.app (heapΣ (@LM_EM_HL _ spinlock_model)) spinlockΣ). 
-  assert (heapGpreS Σ (@LM_EM_HL _ spinlock_model)) as HPreG.
+  set (Σ := gFunctors.app (heapΣ (@LM_EM_HL _ _ spinlock_model)) spinlockΣ). 
+  assert (heapGpreS Σ (@LM_EM_HL _ _ spinlock_model)) as HPreG.
   { apply _. }
-  eapply (simple_simulation_adequacy_terminate_ftm Σ NotStuck _ ([2; 2] : fmstate spinlock_model_impl) ∅)
+  unshelve eapply (simple_simulation_adequacy_terminate_ftm Σ NotStuck _ ([2; 2] : fmstate spinlock_model_impl) _ ∅)
   =>//.
+  - done. 
   - eapply valid_state_evolution_finitary_fairness_simple.
     intros ?. simpl.
     apply (spinlock_model_finitary s1).    
